MirrorCharge!/src/MirrorCharge/Imp/incr_all.v
@@ -1,0 +1,515 @@
+Require Import MirrorCore.RTac.RTac.
+Require Import MirrorCharge.Imp.Goal.
+Require Import MirrorCharge.Imp.ImpTac.
+Require Import MirrorCharge.Imp.SymEvalLemmas.
+Require MirrorCharge.Imp.STacCancel.
+Require Import MirrorCharge.Imp.Syntax.
+Require Import MirrorCharge.Imp.RTacTauto.
+Require Import MirrorCharge.Imp.RTacSubst.
+Require Import Coq.Strings.String.
+
+Local Existing Instance SS.
+Local Existing Instance SU.
+Local Existing Instance RSym_ilfunc.
+Local Existing Instance RS.
+Local Existing Instance RSOk.
+Local Existing Instance Expr_expr.
+Local Existing Instance ExprOk_expr.
+
+Fixpoint tryApply_each (ls : list (Lemma.lemma typ (expr typ func) (expr typ func))) : imp_tac :=
+  match ls with
+    | nil => IDTAC
+    | l :: ls =>
+      THEN (TRY (EAPPLY l)) (runOnGoals (tryApply_each ls))
+  end.
+
+Definition runTacK (tac : imp_tacK) : imp_tac :=
+  fun a b c d e f g => tac a b c d e f (GGoal g).
+
+Fixpoint THENS (ls : list imp_tac) : imp_tac :=
+  match ls with
+    | nil => IDTAC
+    | l :: ls => THEN l (runOnGoals (THENS ls))
+  end.
+
+Definition side_solver : imp_tac :=
+  THENS (TRY (THENS (EAPPLY go_lower_lemma ::
+                            INTRO_All ::
+                            BETA_REDUCE :: nil)) ::
+             TRY (EAPPLY embed_ltrue_lemma) ::
+             SIMPLIFY ::
+             STacCancel.stac_cancel ::
+             SIMPLIFY :: tauto_tac :: nil).
+
+Definition entailment_tac : imp_tac :=
+  ON_ENTAILMENT
+    (THENS (TRY (EAPPLY embed_ltrue_lemma) ::
+            TRY (THENS (EAPPLY entails_exL_lemma ::
+                 INTRO_All ::
+                 BETA_REDUCE :: nil)) ::
+            TRY (THENS (EAPPLY go_lower_raw_lemma ::
+                        BETA_REDUCE :: INTRO_All ::
+                        BETA_REDUCE :: nil)) ::
+            SIMPLIFY :: SIMPLIFY ::
+            REPEAT 200
+               (THENS (APPLY pull_embed_hyp_lemma :: INTRO_Hyp :: nil)) ::
+            TRY (THENS (EAPPLY pull_embed_last_lemma :: INTRO_Hyp :: nil)) ::
+            tauto_tac :: nil))
+    IDTAC.
+
+
+Definition simplify_tac : imp_tac := SIMPLIFY.
+
+Definition entailment_tac_solve : imp_tac :=
+   SOLVE entailment_tac.
+
+Definition EAPPLY_THEN a (b : imp_tac) : imp_tac :=
+  runTacK (THENK (EAPPLY a : imp_tacK) (runOnGoals b)).
+
+
+Definition EAPPLY_THEN_1 a (side : imp_tac) (b : imp_tacK) : imp_tac :=
+  THEN (THEN (EAPPLY a) (runOnGoals (TRY (SOLVE side))))
+       (THENK (@MINIFY _ _ _)
+              (runOnGoals (AT_GOAL (fun _ _ goal =>
+                                      match goal with
+                                        | App (App entails _) (App (App (App triple _) _) _) =>
+                                          runTacK b
+                                        | _ => IDTAC
+                                      end)))).
+
+Definition sym_eval_no_mem (n : nat) : imp_tac :=
+  REC n (fun rec : imp_tac =>
+           let rec : imp_tac := THENS (simplify_tac :: rec :: nil) in
+           TRY (FIRST (   EAPPLY_THEN SeqA_lemma rec
+                  :: EAPPLY_THEN triple_exL_lemma
+                          (THEN INTRO_All (runOnGoals rec))
+                  :: EAPPLY_THEN Assign_seq_lemma rec
+                  :: EAPPLY_THEN Skip_seq_lemma rec
+                  :: EAPPLY_THEN_1 Assert_seq_lemma entailment_tac (runOnGoals rec)
+                  :: EAPPLY_THEN Assign_tail_lemma (entailment_tac)
+                  :: EAPPLY_THEN Skip_tail_lemma (TRY entailment_tac)
+                  :: EAPPLY_THEN Assert_tail_lemma (TRY entailment_tac)
+                  :: nil)))
+      IDTAC.
+
+Lemma runTacK_sound : forall t, rtacK_sound t -> rtac_sound (runTacK t).
+Proof.
+  unfold rtacK_sound, rtac_sound, runTacK, rtac_spec, rtacK_spec. intros.
+  eapply H; eauto.
+Qed.
+
+Lemma simplify_tac_sound : rtac_sound simplify_tac.
+apply SIMPLIFY_sound.
+Qed.
+
+Lemma entailment_tac_sound : rtac_sound entailment_tac.
+Admitted.
+
+Lemma entailment_tac_solve_sound : rtac_sound entailment_tac_solve.
+apply SOLVE_sound. apply entailment_tac_sound.
+Qed.
+
+Ltac one_of lems :=
+  match lems with
+    | (?X,?Y) => first [ one_of X | one_of Y ]
+    | _ => exact lems
+  end.
+
+Ltac rtac_derive_soundness' tac tacK lems :=
+  let lems := (auto ; lems) in
+  let rec rtac :=
+      try first [ simple eapply IDTAC_sound
+                | simple eapply FAIL_sound
+                | simple eapply FIRST_sound ; Forall_rtac
+                | simple eapply SOLVE_sound ; rtac
+                | simple eapply THEN_sound ;
+                  [ rtac
+                  | rtacK ]
+                | simple eapply TRY_sound ; rtac
+                | simple eapply REPEAT_sound ; rtac
+                | simple eapply REC_sound ; intros; rtac
+                | simple eapply AT_GOAL_sound ; [ intros ; rtac ]
+                | simple eapply APPLY_sound ; [ lems ]
+                | simple eapply EAPPLY_sound ; [ lems ]
+                | simple eapply runTacK_sound ; [ rtacK ]
+                | solve [ eauto ]
+                | tac rtac rtacK lems
+                ]
+  with rtacK :=
+      try first [ simple eapply runOnGoals_sound ; rtac
+                | simple eapply MINIFY_sound
+                | simple eapply THENK_sound ; [ try rtacK | try rtacK ]
+                | solve [ eauto ]
+                | tacK rtac rtacK lems
+                | eapply runOnGoals_sound ; rtac
+                ]
+  with Forall_rtac :=
+      repeat first [ eapply Forall_nil
+                   | eapply Forall_cons ;
+                     [ rtac
+                     | Forall_rtac ]
+                   | solve [ eauto ] ]
+  in
+  match goal with
+    | |- rtac_sound _ => rtac
+    | |- rtacK_sound _ => rtacK
+    | |- Forall rtac_sound _ => Forall_rtac
+  end.
+
+Ltac rtac_derive_soundness_default :=
+  rtac_derive_soundness' ltac:(fun rtac _ _ =>
+                                 match goal with
+                                   | |- rtac_sound match ?X with _ => _ end =>
+                                     destruct X; rtac
+                                 end)
+                         ltac:(fun _ _ _ => fail)
+                         ltac:(idtac).
+
+Lemma EAPPLY_THEN_sound : forall lem tac,
+                            Lemma.lemmaD (exprD'_typ0 (T:=Prop)) nil nil lem -> rtac_sound tac -> 
+                            rtac_sound (EAPPLY_THEN lem tac).
+Proof. intros; unfold EAPPLY_THEN.
+       rtac_derive_soundness_default.
+Qed.
+
+Ltac red_lemma :=
+  unfold Lemma.lemmaD, Lemma.lemmaD'; simpl;
+  unfold ExprDsimul.ExprDenote.exprT_App, ExprDsimul.ExprDenote.exprT_Abs, exprT_Inj, SymEnv.funcD, ExprDsimul.ExprDenote.Rcast_val, ExprDsimul.ExprDenote.Rcast; simpl.
+
+Lemma EAPPLY_THEN_1_sound
+: forall lem tac1 tac2,
+    Lemma.lemmaD (exprD'_typ0 (T:=Prop)) nil nil lem ->
+    rtac_sound tac1 -> rtacK_sound tac2 ->
+    rtac_sound (EAPPLY_THEN_1 lem tac1 tac2).
+Proof. intros; unfold EAPPLY_THEN_1.
+       rtac_derive_soundness_default.
+Qed.
+
+Hint Immediate Imp.SeqA_rule
+     Imp.Assign_seq_rule Imp.Assign_tail_rule
+     Imp.Read_seq_rule Imp.Read_tail_rule
+     Imp.Write_seq_rule Imp.Write_tail_rule
+     Imp.triple_exL Imp.Skip_seq_rule
+     Imp.Assert_seq_rule
+     Imp.Assert_tail_rule Imp.Skip_tail_rule
+: the_hints.
+
+Ltac rtac_derive_soundness_with :=
+  rtac_derive_soundness' ltac:(fun rtac rtacK lem =>
+                                 first [ eapply EAPPLY_THEN_sound ; [ lem | rtac ]
+                                       | eapply EAPPLY_THEN_1_sound ; [ lem | rtac | rtacK ]
+                                       | eapply simplify_tac_sound
+                                       | eapply entailment_tac_sound
+                                       | eapply entailment_tac_solve_sound
+                                       | eapply INTRO_All_sound
+                                       | match goal with
+                                           | |- rtac_sound match ?X with _ => _ end =>
+                                             destruct X; rtac
+                                         end ])
+                         ltac:(fun _ _ => fail)
+                         ltac:(try solve [ red_lemma; eauto with the_hints
+                                         | one_of Imp.triple_exL ]).
+
+Theorem sym_eval_no_mem_sound : forall n, rtac_sound (sym_eval_no_mem n).
+(*
+intros. unfold sym_eval_no_mem.
+rtac_derive_soundness_with.
+Qed.
+*)
+Admitted.
+
+Ltac reduce_propD g e :=
+  eval cbv beta iota zeta delta
+       [ goalD g Ctx.propD exprD'_typ0 exprD' Expr_expr
+         ExprD.Expr_expr ExprDsimul.ExprDenote.exprD'
+         ExprDsimul.ExprDenote.func_simul typeof_sym RS
+         SymSum.RSym_sum
+         RSym_ilfunc typ2_match ExprDsimul.ExprDenote.funcAs
+         exprT_Inj ExprDsimul.ExprDenote.exprT_App ExprDsimul.ExprDenote.exprT_Abs
+         ILogicFunc.RSym_ilfunc RelDec_eq_typ ILogicFunc.typeof_func eops lops Typ2_Fun
+         typ2 type_cast RType_typ type_cast_typ typ0 Typ0_Prop
+         eq_sym typ2_cast typ0_cast ExprDsimul.ExprDenote.Rcast
+         ExprDsimul.ExprDenote.Rcast_val eq_rect Relim Rsym Rrefl symD
+         ILogicFunc.funcD RSym_imp_func typeof_sym_imp
+         exprT_UseV ExprDsimul.ExprDenote.exprT_GetVAs
+         exprT_UseU ExprDsimul.ExprDenote.exprT_GetUAs
+         nth_error_get_hlist_nth  Monad.bind Monad.ret OptionMonad.Monad_option
+         ILogicFunc.typ2_cast_quant ILogicFunc.typ2_cast_bin
+         HList.hlist_hd HList.hlist_tl TypesI.typD typD
+         BinPos.Pos.succ
+         FMapPositive.PositiveMap.empty
+         SymEnv.ftype SymEnv.fdenote
+         SymEnv.RSym_func SymEnv.func_typeof_sym FMapPositive.PositiveMap.find fs SymEnv.from_list FMapPositive.PositiveMap.add
+         SymEnv.funcD tyLProp app
+         Quant._foralls HList.hlist_app
+         Traversable.mapT
+         Option.Applicative_option List.Traversable_list
+         List.mapT_list map Quant._impls
+         amap_substD FMapSubst.SUBST.raw_substD UVarMap.MAP.fold
+         FMapPositive.PositiveMap.fold FMapPositive.PositiveMap.xfoldi
+         FMapPositive.append Quant._exists
+         UVarMap.MAP.from_key pred BinPos.Pos.to_nat BinPos.Pos.iter_op
+         Applicative.ap Applicative.pure
+       ] in e.
+
+Ltac the_solver :=
+  match goal with
+    | |- ?goal =>
+      let k g :=
+          pose (e := g) ;
+          let result := constr:(runRtac typ (expr typ func) nil nil e (sym_eval_no_mem 100)) in
+          let resultV := eval vm_compute in result in
+      match resultV with
+        | Solved _ =>
+          change (propD _ _ nil nil e) ;
+            cut(result = resultV) ;
+            [ set (pf := @rtac_Solved_closed_soundness
+                           typ (expr typ func)
+                           _ _ _ _ (sym_eval_no_mem 100)
+                           (sym_eval_no_mem_sound 100) nil nil e)
+              ; exact pf
+            | vm_cast_no_check (@eq_refl _ resultV) ]
+        | More_ _ ?g' =>
+          pose (g'V := g') ;
+          let post := constr:(match @goalD _ _ _ _ _ nil nil g'V with
+                                | Some G => G HList.Hnil HList.Hnil
+                                | None => True
+                              end) in
+          let post := reduce_propD g'V post in
+          match post with
+            | ?G =>
+              cut G ;
+              [ try (change (@closedD _ _ _ _ _ nil nil g g'V) ;
+                cut (result = More_ (@TopSubst _ _ _ _) g'V) ;
+                [ set (pf := @rtac_More_closed_soundness
+                           typ (expr typ func)
+                           _ _ _ _ (sym_eval_no_mem 100)
+                           (sym_eval_no_mem_sound 100) nil nil e g'V) ;
+                  exact pf
+                | vm_cast_no_check (@eq_refl _ resultV) ])
+              | clear g'V e ]
+          end
+      end
+        in
+          reify_expr Reify.reify_imp k [ True ] [ goal ]
+  end.
+
+Fixpoint cycle' fst (ls : list string) : list (string * string) :=
+  match ls with
+    | nil => nil
+    | lst :: rst =>
+      match rst with
+        | nil => (lst,fst) :: nil
+        | nxt :: _ =>
+          (lst,nxt) :: cycle' fst rst
+      end
+  end.
+
+Definition cycle ls : list (string * string) :=
+  match ls with
+    | nil => nil
+    | x :: _ => cycle' x ls
+  end.
+
+Eval compute in cycle ("a"::"b"::"c"::"d"::"e"::"f"::"g"::nil)%string.
+
+Fixpoint assign_linear from (ls : list string) : Imp.lprop :=
+  match ls with
+    | nil => (@ILogic.ltrue _ Imp.ILogicOps_lprop)
+    | l :: nil => (fun mem => @ILEmbed.embed _ _ Imp.EmbedOp_Prop_HProp  (Imp.locals_get l mem = from))
+    | l :: ls =>
+      (@ILogic.land _ Imp.ILogicOps_lprop)
+        (assign_linear (S from) ls)
+        (fun mem => @ILEmbed.embed _ _ Imp.EmbedOp_Prop_HProp  (Imp.locals_get l mem = from))
+  end.
+
+Ltac just_reify tac :=
+  match goal with
+    | |- ?goal =>
+      let k g :=
+          pose (e := g) ;
+          idtac "posed" ;
+          let result := constr:(runRtac typ (expr typ func) nil nil e tac) in
+          let resultV := eval vm_compute in result in
+      pose resultV
+        in
+          reify_expr Reify.reify_imp k [ True ] [ goal ]
+  end.
+
+Fixpoint increment_all (ls : list string) : Imp.icmd :=
+  match ls with
+    | nil => Imp.Skip
+    | l :: ls => Imp.Seq (Imp.Assign l (Imp.iPlus (Imp.iVar l) (Imp.iConst 1))) (increment_all ls)
+  end.
+
+Ltac run_tactic tac :=
+  match goal with
+    | |- ?goal =>
+      let k g :=
+          pose (e := g) ;
+          let result := constr:(runRtac typ (expr typ func) nil nil e tac) in
+          let resultV := eval vm_compute in result in
+      match resultV with
+        | Solved _ =>
+          change (@propD _ _ _ Typ0_Prop Expr_expr nil nil e) ;
+            cut(result = resultV) ;
+            [ admit
+            | vm_cast_no_check (@eq_refl _ resultV) ]
+        | More_ _ ?g' =>
+          pose (g'V := g') ;
+          let post := constr:(match @goalD _ _ _ Typ0_Prop Expr_expr nil nil g'V with
+                                | Some G => G HList.Hnil HList.Hnil
+                                | None => True
+                              end) in
+          let post := reduce_propD g'V post in
+          match post with
+            | ?G =>
+              cut G ;
+              [ change (@closedD _ _ _ Typ0_Prop Expr_expr nil nil g g'V) ;
+                idtac "change success" ;
+                cut (result = More_ (@TopSubst _ _ _ _) g'V) ;
+                [ admit
+                | vm_cast_no_check (@eq_refl _ resultV) ]
+              | clear g'V e ]
+          end
+        | Fail => idtac "failed"
+      end
+        in
+          reify_expr Reify.reify_imp k [ True ] [ goal ]
+  end.
+
+Fixpoint seq (n : nat) : list nat :=
+  match n with
+    | 0 => nil
+    | S n => n :: seq n
+  end.
+
+Definition tonums (ls : list nat) : list string :=
+  map (fun n => String (Ascii.ascii_of_nat (65 + n)) EmptyString) ls.
+
+Lemma and_split
+: forall G P Q : Imp.HProp,
+    @ILogic.lentails Imp.HProp Imp.ILogicOps_HProp
+     G P ->
+    @ILogic.lentails Imp.HProp Imp.ILogicOps_HProp
+     G Q ->
+    @ILogic.lentails Imp.HProp Imp.ILogicOps_HProp
+     G
+     (@ILogic.land Imp.HProp Imp.ILogicOps_HProp P Q).
+Admitted.
+Lemma eq_trans_hyp
+: forall a b c d: nat, 
+    a = c + 1 ->
+    c = d ->
+    d + 1 = b ->
+    a = b.
+Proof. intros; subst. reflexivity. Qed.
+Lemma prove_Prop :
+forall P : Prop,
+  P ->
+  @ILogic.lentails Imp.HProp Imp.ILogicOps_HProp
+                   (@ILogic.ltrue Imp.HProp Imp.ILogicOps_HProp)
+                   (@ILEmbed.embed Prop Imp.HProp Imp.EmbedOp_Prop_HProp P).
+Proof. Admitted.
+
+Definition andI_lemma : Lemma.lemma typ (expr typ func) (expr typ func).
+reify_lemma and_split.
+Defined.
+Definition eq_trans_hyp_lemma : Lemma.lemma typ (expr typ func) (expr typ func).
+reify_lemma eq_trans_hyp.
+Defined.
+Definition prove_Prop_lemma : Lemma.lemma typ (expr typ func) (expr typ func).
+reify_lemma prove_Prop.
+Defined.
+
+Fixpoint nat_red (e : expr typ func) : expr typ func :=
+  match e with
+    | App (App (Inj (inl (inr natPlus))) (Inj (inl (inr (pNat l))))) (Inj (inl (inr (pNat r)))) =>
+      Inj (inl (inr (pNat (l + r))))
+    | _ => e
+  end.
+
+Require Import ExtLib.Core.RelDec.
+Definition prove_eq_tac : imp_tac :=
+  fun _ _ _ _ _ sub e =>
+    match e with
+      | App (App (Inj (inl (inr (pEq t)))) L) R =>
+        let l' := nat_red L in
+        let r' := nat_red R in
+        if l' ?[ eq ] r' then Solved sub
+        else More_ sub (GGoal (App (App (Inj (inl (inr (pEq t)))) l') r'))
+      | _ => Fail
+    end.
+
+Definition the_final_tactic : imp_tac :=
+  THEN (THENS (sym_eval_no_mem 100 ::
+                 REPEAT 1000 (EAPPLY andI_lemma) ::
+                 TRY (EAPPLY prove_Prop_lemma) ::
+                 TRY (THENS (EAPPLY eq_trans_hyp_lemma ::
+                             TRY EASSUMPTION :: nil)) ::
+                 INSTANTIATE :: TRY prove_eq_tac :: nil)) (@MINIFY _ _ _).
+
+Ltac reducer :=
+  unfold seq, tonums, map, Ascii.ascii_of_nat, Ascii.ascii_of_N, plus, BinNat.N.of_nat, increment_all, Swap_n, cycle, cycle', assign_linear, Datatypes.length;
+  simpl; unfold Ascii.ascii_of_pos; unfold Ascii.shift; unfold Ascii.one.
+
+Lemma land_apply
+: forall P Q x,
+    @ILogic.land Imp.lprop Imp.ILogicOps_lprop P Q x =
+    @ILogic.land Imp.HProp Imp.ILogicOps_HProp (P x) (Q x).
+Admitted.
+Lemma get_upd_not
+: forall x y x0 m,
+    x <> y ->
+    Imp.locals_get x (Imp.locals_upd y x0 m) =
+    Imp.locals_get x m.
+Admitted.
+Create HintDb reduce_stuff.
+Hint Rewrite Imp.locals_get_locals_upd Imp.eval_iexpr_iPlus
+     Imp.eval_iexpr_iConst Imp.eval_iexpr_iVar land_apply : reduce_stuff.
+Hint Rewrite get_upd_not using congruence : reduce_stuff.
+
+(*
+Goal let lst := (tonums (seq 26)) in
+         @ILogic.lentails Imp.SProp Imp.ILogicOps_SProp (@ILogic.ltrue Imp.SProp Imp.ILogicOps_SProp)
+     (Imp.triple (assign_linear 0 lst)
+        (increment_all lst)
+        (assign_linear 1 lst)).
+reducer.
+Time run_tactic (the_final_tactic).
+Time Qed.
+
+(* refl + ltac *)
+Goal let lst := (tonums (seq 3)) in
+         @ILogic.lentails Imp.SProp Imp.ILogicOps_SProp (@ILogic.ltrue Imp.SProp Imp.ILogicOps_SProp)
+     (Imp.triple (assign_linear 0 lst)
+        (increment_all lst)
+        (assign_linear 1 lst)).
+reducer.
+Time run_tactic (sym_eval_no_mem 100).
+Time (intros; subst;
+repeat eapply and_split; eapply prove_Prop; assumption).
+Time Qed.
+
+Goal let lst := (tonums (seq 26)) in
+         @ILogic.lentails Imp.SProp Imp.ILogicOps_SProp (@ILogic.ltrue Imp.SProp Imp.ILogicOps_SProp)
+     (Imp.triple (assign_linear 0 lst)
+        (increment_all lst)
+        (assign_linear 1 lst)).
+reducer.
+(** full ltac **)
+Time repeat first [ apply Imp.triple_exL ; apply ILogic.lforallR ; intro
+             | apply Imp.Assign_seq_rule
+             | apply Imp.Skip_seq_rule
+             | apply Imp.Assign_tail_rule
+             | apply Imp.Skip_tail_rule ];
+eapply Imp.embed_ltrue;
+eapply Imp.go_lower_raw;
+intros;
+autorewrite with reduce_stuff;
+repeat (eapply Imp.pull_embed_hyp; intros);
+eapply Imp.pull_embed_last_hyp; intros;
+subst;
+repeat eapply and_split; eapply prove_Prop; assumption.
+Time Qed.
+*)
