MirrorCharge!/src/MirrorCharge/Imp/incr_all_ltac.v
@@ -1,0 +1,22 @@
+Require Import incr_all.
+
+Goal let lst := (tonums (seq NNN)) in
+         @ILogic.lentails Imp.SProp Imp.ILogicOps_SProp (@ILogic.ltrue Imp.SProp Imp.ILogicOps_SProp)
+     (Imp.triple (assign_linear 0 lst)
+        (increment_all lst)
+        (assign_linear 1 lst)).
+reducer.
+Time repeat first [ apply Imp.triple_exL ; apply ILogic.lforallR ; intro
+             | apply Imp.Assign_seq_rule
+             | apply Imp.Skip_seq_rule
+             | apply Imp.Assign_tail_rule
+             | apply Imp.Skip_tail_rule ];
+eapply Imp.embed_ltrue;
+eapply Imp.go_lower_raw;
+intros;
+autorewrite with reduce_stuff;
+repeat (eapply Imp.pull_embed_hyp; intros);
+eapply Imp.pull_embed_last_hyp; intros;
+subst;
+repeat eapply and_split; eapply prove_Prop; assumption.
+Time Qed.
