MirrorCharge!/src/MirrorCharge/Imp/incr_all_mixed.v
@@ -1,0 +1,12 @@
+Require Import incr_all.
+
+Goal let lst := (tonums (seq NNN)) in
+         @ILogic.lentails Imp.SProp Imp.ILogicOps_SProp (@ILogic.ltrue Imp.SProp Imp.ILogicOps_SProp)
+     (Imp.triple (assign_linear 0 lst)
+        (increment_all lst)
+        (assign_linear 1 lst)).
+reducer.
+Time run_tactic (incr_all.sym_eval_no_mem 100).
+Time (intros; subst;
+repeat eapply and_split; eapply prove_Prop; assumption).
+Time Qed.
