MirrorCharge!/src/MirrorCharge/Imp/incr_all_refl.v
@@ -1,0 +1,11 @@
+Require Import incr_all.
+
+(* full refl *)
+Goal let lst := (tonums (seq NNN)) in
+         @ILogic.lentails Imp.SProp Imp.ILogicOps_SProp (@ILogic.ltrue Imp.SProp Imp.ILogicOps_SProp)
+     (Imp.triple (assign_linear 0 lst)
+        (increment_all lst)
+        (assign_linear 1 lst)).
+reducer.
+Time run_tactic (the_final_tactic).
+Time Qed.
